examples/Hoare/LogicTac.v
@@ -1,3 +1,5 @@
+Require Import ExtLib.Tactics.
+Require Import MirrorCore.Util.Forwardy.
 Require Import MirrorCore.TypesI.
 Require Import MirrorCore.SymI.
 Require Import MirrorCore.Views.FuncView.
@@ -7,6 +9,7 @@ Require Import MirrorCore.Lambda.Expr.
 Require Import MirrorCore.Lambda.Ptrns.
 Require Import MirrorCore.Lambda.RedAll.
 Require Import MirrorCore.Lambda.ExprVariables.
+Require Import MirrorCore.Lambda.ExprTac.
 Require Import MirrorCore.Lambda.Rtac.
 Require Import McExamples.Hoare.Imp.
 Require Import McExamples.Hoare.ILogicFunc.
@@ -15,9 +18,9 @@ Section parametric.
   Context {typ func : Type}.
   Context {RType_typ : RType typ}.
   Context {RTypeOk_typ : RTypeOk}.
-  Context {Typ2_RFun : Typ2 _ RFun}.
+  Context {Typ2_RFun : Typ2 RType_typ RFun}.
   Context {Typ2Ok_RFun : Typ2Ok Typ2_RFun}.
-  Context {Typ0_Prop : Typ0 _ Prop}.
+  Context {Typ0_Prop : Typ0 RType_typ Prop}.
   Context {Typ0Ok_Prop : Typ0Ok Typ0_Prop}.
   Context {RSym_func : RSym func}.
   Context {RSymOk_func : RSymOk RSym_func}.
@@ -25,7 +28,14 @@ Section parametric.
   Context {FV : FuncView func (ilfunc typ)}.
   Variable ilo : @logic_ops  _ _.
   Variable eo : @embed_ops  _ _.
+  Context {iloOk : logic_opsOk ilo}.
   Context {FVO : FuncViewOk FV RSym_func (RSym_ilfunc (RelDec_eq_typ) ilo eo _ _) }.
+
+  Context {ilo_Prop : ilo (typ0 (F:=Prop)) =
+                      lSome match eq_sym (typ0_cast (F:=Prop)) in _ = X
+                                  return ILogic.ILogicOps X with
+                            | eq_refl => ILogic.ILogicOps_Prop
+                            end}.
 
   Definition bin_op {T U V W} (f : T -> U -> V -> W)
              (t : ptrn func T) (l : ptrn (expr typ func) U) (r : ptrn (expr typ func) V)
@@ -35,7 +45,13 @@ Section parametric.
 
   Definition ptrn_ok_bin_op {T U V W} f t l r :
     ptrn_ok t -> ptrn_ok l -> ptrn_ok r -> ptrn_ok (@bin_op T U V W f t l r).
-  Proof. Admitted.
+  Proof.
+    intros. unfold bin_op.
+    repeat first [ eassumption
+                 | eapply ptrn_ok_appl
+                 | eapply ptrn_ok_inj
+                 | eapply ptrn_ok_pmap ].
+  Qed.
 
   Definition ptrn_entails {T U V}
              (t : ptrn typ V)
@@ -59,17 +75,17 @@ Section parametric.
   Definition intro_ptrn_all : ptrn (expr typ func) (OpenAs typ (expr typ func)) :=
     por
       (appl (inj (ptrn_view _ (fptrn_lforall get (fun t => pmap (fun _ => t) ignore))))
-            (pmap (fun body t => AsAl t (fun arg => Red.beta (lift 0 1 (App body arg)))) get))
+            (pmap (fun body t => SimpleOpen_to_OpenAs (sAsAl t body)) get))
       (ptrn_entails get (pmap (fun G t => (G,t)) get)
                     (appl (inj (ptrn_view _ (fptrn_lforall get (fun t => pmap (fun _ => t) ignore))))
                           (pmap (fun body t Gt =>
                                    let '(G,l) := Gt in
                                    AsAl t (fun arg =>
-                                             App (App (Inj (f_insert (ilf_forall t l))) (lift 0 1 G))
-                                                 (Red.beta (lift 0 1 (App body arg))))) get))).
+                                             App (App (Inj (f_insert (ilf_entails l))) G)
+                                                 (Red.beta (App body arg)))) get))).
 
-  Definition intro_ptrn_hyp : ptrn (expr typ func) (OpenAs typ (expr typ func)) :=
-    bin_op (fun _ P Q => AsHy P Q)
+  Definition intro_ptrn_hyp : ptrn (expr typ func) (SimpleOpen typ func) :=
+    bin_op (fun _ P Q => sAsHy P Q)
            (ptrn_view _ (fptrn_limpl ignore)) get get.
 
   Ltac solve_ok :=
@@ -86,9 +102,6 @@ Section parametric.
   Local Existing Instance RSym_func.
   Local Existing Instance RType_typ.
 
-  Require Import ExtLib.Tactics.
-  Require Import MirrorCore.Util.Forwardy.
-
   Lemma exprD'_App_both_cases : forall tus tvs tx ty f x fD xD,
       exprD' tus tvs (typ2 tx ty) f = Some fD ->
       exprD' tus tvs tx x = Some xD ->
@@ -102,18 +115,45 @@ Section parametric.
 
   Ltac solve_stuff :=
     try lazymatch goal with
-  | |- ptrn_ok _ => solve_ok
-  | |- _ =>
-    match goal with
-    | H : Succeeds _ _ _ |- _ =>
-      first [ simple eapply Succeeds_appl in H; [ forward_reason; subst; solve_stuff | clear H; solve_ok | clear H; solve_ok ]
-            | simple eapply Succeeds_pmap in H; [ forward_reason; subst; solve_stuff | clear H; solve_ok ]
-            | simple eapply Succeeds_get in H; subst; solve_stuff
-            | simple eapply Succeeds_inj in H; [ forward_reason; subst; solve_stuff | clear H; solve_ok ]
-            | (eapply Succeeds_ptrn_view in H;
-               [ | solve [ eauto with typeclass_instances ] | clear H ]); [ forward_reason; subst; solve_stuff | ] ]
-    end
-  end.
+        | |- ptrn_ok _ => solve_ok
+        | |- _ =>
+          match goal with
+          | H : Succeeds _ _ _ |- _ =>
+            first [ simple eapply Succeeds_appl in H; [ forward_reason; subst; solve_stuff | clear H; solve_ok | clear H; solve_ok ]
+                  | simple eapply Succeeds_pmap in H; [ forward_reason; subst; solve_stuff | clear H; solve_ok ]
+                  | simple eapply Succeeds_get in H; subst; solve_stuff
+                  | simple eapply Succeeds_inj in H; [ forward_reason; subst; solve_stuff | clear H; solve_ok ]
+                  | (eapply Succeeds_ptrn_view in H;
+                     [ | solve [ eauto with typeclass_instances ] | clear H ]); [ forward_reason; subst; solve_stuff | ] ]
+          end
+        end.
+
+  Theorem Succeeds_ptrn_entails {T U V} e t a b r
+  : ptrn_ok a -> ptrn_ok b -> ptrn_ok t ->
+    Succeeds e (@ptrn_entails T U V t a b) r ->
+    exists te ta tb tr ar br,
+      e = App (App (Inj (f_insert (ilf_entails te))) ta) tb /\
+      r = br (ar tr) /\
+      Succeeds te t tr /\
+      Succeeds ta a ar /\
+      Succeeds tb b br.
+  Proof.
+    unfold ptrn_entails. intros.
+    solve_stuff; try solve_ok; eauto using fptrn_lentails_ok.
+    eapply (@s_elim _ _ _ _ _ (@SucceedsE_fptrn_lentails _ _ _ _ _)) in H5.
+    simpl in H5. forward_reason.
+    subst.
+    do 6 eexists. split; [ reflexivity | ].
+    split; [ reflexivity | ].
+    eauto.
+  Qed.
+
+  Let Expr_expr := @Expr_expr _ _ RType_typ _ RSym_func.
+  Local Existing Instance Expr_expr.
+  Let ExprOk_expr : ExprOk Expr_expr := @ExprOk_expr _ _ RType_typ _ RSym_func _ _ _.
+  Local Existing Instance ExprOk_expr.
+
+  Local Opaque Red.beta.
 
   Theorem intro_ptrn_all_sound : open_ptrn_sound intro_ptrn_all.
   Proof.
@@ -123,11 +163,13 @@ Section parametric.
     destruct H.
     - solve_stuff.
       eapply (@s_elim _ _ _ _ _ (@SucceedsE_fptrn_lforall _ _ _ _ _ _ _ _)) in H1.
+      2: solve_ok.
       simpl in H1.
       forward_reason. subst.
+      eapply SimpleOpen_to_OpenAs_sound; eauto.
       solve_stuff.
       + clear H x1.
-        Opaque Red.beta.
+        red.
         unfold Ctx.propD, exprD'_typ0. simpl. intros.
         forwardy.
         inv_all. subst.
@@ -135,27 +177,113 @@ Section parametric.
         destruct (ilo x2) eqn:?; try congruence.
         forwardy. inv_all. subst.
         generalize y. intro. clear H.
-        eapply typ2_inj in y.
+        eapply typ2_inj in y; [ | eassumption ].
         unfold Rty in y. destruct y; subst.
-        generalize (Red.beta_sound tus (tvs ++ x4 :: nil) (lift 0 1 (App x3 e')) (typ0 (F:=Prop))).
-        simpl lift.
-        (*
-      erewrite exprD'_App_both_cases.
-      4: eassumption.
-         *)
-        admit.
-        eassumption.
-      + solve_ok.
-    - admit.
-  Admitted.
+        eexists; split; [ eassumption | ].
+        assert (i = match
+                  eq_sym (typ0_cast (F:=Prop)) in (_ = X)
+                  return (ILogic.ILogicOps X)
+                with
+                | eq_refl => ILogic.ILogicOps_Prop
+                end).
+        { clear - ilo_Prop Heql.
+          revert Heql. change_rewrite ilo_Prop.
+          inversion 1. reflexivity. }
+        subst. clear - RTypeOk_typ.
+        unfold castD. simpl.
+        unfold typ2_cast_quant, AbsAppI.exprT_App.
+        generalize dependent (typ0_cast (F:=Prop)).
+        generalize dependent (typ2_cast x4 (typ0 (F:=Prop))).
+        generalize dependent (typ2_cast (typ2 x4 (typ0 (F:=Prop))) (typ0 (F:=Prop))).
+        rewrite (UIP_refl y0); clear y0; simpl.
+        revert x1.
+        generalize ((typD (typ2 x4 (typ0 (F:=Prop))))).
+        generalize (typD (typ2 (typ2 x4 (typ0 (F:=Prop))) (typ0 (F:=Prop)))).
+        generalize (typD (typ0 (F:=Prop))).
+        intros; subst; simpl in *.
+        assumption.
+    - eapply Succeeds_ptrn_entails in H;
+        try solve_ok; eauto using fptrn_lentails_ok, fptrn_lforall_ok.
+      forward_reason; subst.
+      solve_stuff;
+        try solve_ok; eauto using fptrn_lentails_ok, fptrn_lforall_ok.
+      eapply (@s_elim _ _ _ _ _ (SucceedsE_fptrn_lforall _ _ _ _ _)) in H3;
+        try solve_ok; eauto using fptrn_lentails_ok, fptrn_lforall_ok.
+      simpl in H3. forward_reason. subst.
+      solve_stuff. clear ilo_Prop.
+      clear H. destruct x4. simpl.
+      unfold Ctx.propD, exprD'_typ0. simpl.
+      intros.
+      forwardy; inv_all; subst.
+      assert (x2 = x0 /\ x = x11 /\ x7 = typ2 x3 x11 /\ x0 = x11).
+      { clear - H H3 RTypeOk_typ Typ2Ok_RFun.
+        unfold symAs in *.
+        simpl in *.
+        destruct (ilo x2); try congruence.
+        destruct (ilo x0); try congruence.
+        forwardy. clear H2 H1 H H0.
+        apply typ2_inj in y; eauto.
+        eapply typ2_inj in y0; eauto.
+        destruct y; destruct y0.
+        eapply typ2_inj in H2; eauto.
+        unfold Rty in *. destruct H2.
+        subst. subst.
+        tauto. }
+      destruct H2 as [ ? [ ? [ ? ? ] ] ]; subst.
+      eapply exprD'_weakenV with (Expr_expr:=Expr_expr)(tvs':=x3::nil) in H6; eauto.
+      eapply exprD'_weakenV with (Expr_expr:=Expr_expr)(tvs':=x3::nil) in H4; eauto.
+      forward_reason.
+      erewrite ExprTac.exprD'_AppL; eauto.
+      Focus 2.
+      erewrite ExprTac.exprD'_AppR; eauto.
+      2: eapply H4.
+      red_exprD.
+      rewrite <- (@fv_compat _ _ _ _ _ _ _ FVO).
+      rewrite H. reflexivity.
+      generalize (Red.beta_sound tus (tvs ++ x3 :: nil) (App x1 e') x11).
+      erewrite exprD'_App_both_cases; eauto.
+      2: eapply H2.
+      intros; forwardy.
+      rewrite H7. eexists; split; [ reflexivity | ].
+      intros.
+      unfold symAs in H, H3. simpl in H, H3.
+      destruct (ilo x11) eqn:Hilo; try congruence.
+      specialize (iloOk x11).
+      rewrite Hilo in iloOk.
+      rewrite type_cast_refl in *; eauto.
+      inv_all; subst.
+      simpl in *.
+      generalize (H6 us vs); clear H6.
+      generalize (H5 us vs); clear H5.
+      generalize (H8 us); clear H8.
+      revert H9.
+      unfold AbsAppI.exprT_App.
+      clear H7 H2 H4 H0.
+      unfold typ2_cast_quant.
+      generalize (typ0_cast (F:=Prop)).
+      generalize (typ2_cast (typ2 x3 x11) x11).
+      generalize (typ2_cast x3 x11).
+      generalize (typ2_cast x11 (typ0 (F:=Prop))).
+      generalize (typ2_cast x11 (typ2 x11 (typ0 (F:=Prop)))).
+      generalize dependent (typD (typ2 x11 (typ2 x11 (typ0 (F:=Prop))))).
+      generalize dependent (typD (typ2 x11 (typ0 (F:=Prop)))).
+      generalize dependent (typD (typ2 (typ2 x3 x11) x11)).
+      generalize dependent (typD (typ2 x3 x11)).
+      generalize dependent (typD (typ0 (F:=Prop))).
+      do 12 intro; subst; simpl.
+      intros.
+      eapply ILogic.lforallR.
+      intros.
+      rewrite (H2 (HList.Hcons x2 HList.Hnil)); clear H2.
+      rewrite (H0 (HList.Hcons x2 HList.Hnil)); clear H0.
+      specialize (H (HList.hlist_app vs (HList.Hcons x2 HList.Hnil))).
+      specialize (H9 x2).
+      rewrite H1 in *.
+      rewrite H. assumption.
+  Qed.
 
   Definition INTRO_all : rtac typ (expr typ func) :=
     INTRO_ptrn intro_ptrn_all.
-
-  Let Expr_expr := @Expr_expr _ _ RType_typ _ RSym_func.
-  Local Existing Instance Expr_expr.
-  Let ExprOk_expr : ExprOk Expr_expr := @ExprOk_expr _ _ RType_typ _ RSym_func _ _ _.
-  Local Existing Instance ExprOk_expr.
 
   Instance RtacSound_INTRO_all : RtacSound INTRO_all.
   Proof.
@@ -163,7 +291,8 @@ Section parametric.
     unfold Expr_expr.
     constructor.
     eapply INTRO_ptrn_sound; eauto.
-    - admit.
+    - unfold intro_ptrn_all.
+      eapply ptrn_ok_por; solve_ok.
     - eapply intro_ptrn_all_sound.
-  Admitted.
+  Qed.
 End parametric.
